Adjust embedding to the newest ML

LN_FOL.v
@@ -4,109 +4,94 @@ From MatchingLogic Require Export Logic
                                   Theories.Sorts
                                   Helpers.FOL_helpers.
 Import MatchingLogic.Syntax.Notations MatchingLogic.DerivedOperators.Notations.
+From Coq Require Import ssreflect ssrfun ssrbool.
 Require Export extralibrary 
                Coq.Program.Wf 
                Lia 
                FunctionalExtensionality
+               Logic.PropExtensionality
                Program.Equality.
 From stdpp Require Import countable.
 Require Export Vector PeanoNat String Arith.Lt.
-Print Pattern.
 
-Ltac break_match_hyp :=
+Ltac separate :=
 match goal with
-| [ H : context [ match ?X with _=>_ end ] |- _] =>
-     match type of X with
-     | sumbool _ _=>destruct X
-     | _=>destruct X eqn:? 
-     end 
+| [H : is_true (andb _ _) |- _] => apply andb_true_iff in H as [?E1 ?E2]
+| |- is_true (andb _ _) => apply andb_true_iff
 end.
 
-Ltac break_match_goal :=
-match goal with
-| [ |- context [ match ?X with _=>_ end ] ] => 
-    match type of X with
-    | sumbool _ _ => destruct X
-    | _ => destruct X eqn:?
-    end
-end.
+Definition vec {A : Set} := @t A.
 
-Definition vec := t.
-
-Lemma Forall_map T n (l : vec T n) : forall (P : T -> Prop) (f : T -> T),
+Lemma Forall_map (T : Set) n (l : vec n) : forall (P : T -> Prop) (f : T -> T),
   (forall x, P x -> P (f x))
 ->
   Forall P l -> Forall P (map f l).
 Proof.
-  induction l; intros; constructor;
+  induction l; intros P f H; constructor;
   inversion H0; subst. auto.
   apply IHl; auto. simpl_existT. subst. auto.
 Qed.
 
-Theorem fold_left_map : forall T Q n (v : vec T n) (App : Q -> T -> Q) (start : Q) f,
-  fold_left App start (map f v) = fold_left (fun Acc x => App Acc (f x)) start v.
+Theorem fold_left_map  (T Q : Set) n (v : vec n) :
+   forall (App : Q -> T -> Q) (start : Q) f,
+  fold_left App start (map f v) = @fold_left T Q (fun Acc x => App Acc (f x)) start _ v.
 Proof.
-  induction v; intros; simpl; auto.
+  induction v; intros App start f; simpl; auto.
 Qed.
 
-(* Theorem fold_left_pointwise : forall T Q R n (v : vec T n) (App : Q -> T -> Q) 
-                                     (start : Q) (f : Q -> Q),
-  f (fold_left App start v) = fold_left (fun Acc x => App Acc (f x)) (f start) v. *)
-
-Lemma map_Forall T n (l : vec T n) : forall (P : T -> Prop) (f : T -> T),
+Lemma map_Forall (T : Set) n (l : vec n) : forall (P : T -> Prop) (f : T -> T),
   (forall x, P (f x) -> P x)
 ->
   Forall P (map f l) -> Forall P l.
 Proof.
-  induction l; intros; constructor;
+  induction l; intros P f H; constructor;
   inversion H0; subst. auto.
   eapply IHl; eauto. simpl_existT. now subst.
 Qed.
 
-Lemma Forall_map_ext T n (l : vec T n) : forall (P : T -> Prop) (f : T -> T),
+Lemma Forall_map_ext (T : Set) n (l : vec n) : forall (P : T -> Prop) (f : T -> T),
   (forall x, In x l -> P x -> P (f x))
 ->
   Forall P l -> Forall P (map f l).
 Proof.
-  induction l; intros; constructor;
+  induction l; intros P f H; constructor;
   inversion H0; subst. auto. apply H. constructor. auto.
-  apply IHl; auto. intros. apply H. constructor 2. auto. auto. simpl_existT. now subst.
+  apply IHl; auto. intros x H1 H2. apply H. constructor 2. auto. auto. simpl_existT. now subst.
 Qed.
 
-Lemma map_Forall_ext T n (l : vec T n) : forall (P : T -> Prop) (f : T -> T),
+Lemma map_Forall_ext (T : Set) n (l : vec n) : forall (P : T -> Prop) (f : T -> T),
   (forall x, In x l -> P (f x) -> P x)
 ->
   Forall P (map f l) -> Forall P l.
 Proof.
-  induction l; intros; constructor;
+  induction l; intros P f H; constructor;
   inversion H0; subst. auto. apply H. constructor; auto. auto.
-  eapply IHl; auto. intros. apply H. constructor 2. auto. exact H2. simpl_existT.
+  eapply IHl; auto. intros x H1 H2. apply H. constructor 2. auto. exact H2. simpl_existT.
   now subst.
 Qed.
 
-Lemma Forall_impl_ext 
-     : ∀ (A : Type) (P Q : A → Prop) n,
-         ∀ l : vec A n, (∀ a : A, In a l -> P a → Q a) → Forall P l → Forall Q l.
+Lemma Forall_impl_ext  (A : Set) (P Q : A → Prop) n (l : vec n) :
+   (∀ a : A, In a l -> P a → Q a) → Forall P l → Forall Q l.
 Proof.
-  induction l; intros; constructor; inversion H0; subst.
+  induction l; intros H H0; constructor; inversion H0; subst.
   apply H. constructor; auto. auto.
-  apply IHl; auto. intros. apply H; auto. constructor 2. auto.
+  apply IHl; auto. intros a H1 H2. apply H; auto. constructor 2. auto.
   simpl_existT. now subst.
 Qed.
 
 Global Hint Constructors Forall : core.
 
 Class funcs_signature :=
-  { funs : Type; funs_eqdec : EqDecision funs; ar_funs : funs -> nat }.
+  { funs : Set; funs_eqdec : EqDecision funs; ar_funs : funs -> nat }.
 
 Coercion funs : funcs_signature >-> Sortclass.
 
 Class preds_signature :=
-  { preds : Type; preds_eqdec : EqDecision preds; ar_preds : preds -> nat }.
+  { preds : Set; preds_eqdec : EqDecision preds; ar_preds : preds -> nat }.
 
 Class FOL_variables :=
   {
-    vars : Type;
+    vars : Set;
     var_eqdec : EqDecision vars;
     var_countable : Countable vars;
     var_fresh : list vars -> vars;
@@ -124,10 +109,10 @@ Section fix_signature.
   Context {Σ_funcs : funcs_signature}.
 
   Unset Elimination Schemes.
-  Inductive term  : Type :=
+  Inductive term  : Set :=
   | bvar : nat -> term
   | fvar : vars -> term
-  | func : forall (f : funs), vec term (ar_funs f) -> term.
+  | func : forall (f : funs), @vec term (ar_funs f) -> term.
   Set Elimination Schemes.
 
   Fixpoint fsubst_term (t0 t : term) (n : vars) : term :=
@@ -152,7 +137,7 @@ Section fix_signature.
 
   Inductive form  : Type :=
   | fal : form
-  | atom : forall (P : preds), vec term (ar_preds P) -> form
+  | atom : forall (P : preds), @vec term (ar_preds P) -> form
   | impl : form  -> form  -> form
   | exs : form  -> form.
 
@@ -172,16 +157,16 @@ Section fix_signature.
     | exs phi => exs (bsubst_form phi t (S n))
     end.
 
-  Inductive ForallT {A : Type} (P : A -> Type) : forall {n}, t A n -> Type :=
-  | Forall_nil : ForallT P (@Vector.nil A)
-  | Forall_cons : forall n (x : A) (l : t A n), P x -> ForallT P l -> ForallT P (@Vector.cons A x n l).
+  Inductive ForallT {A : Set} (P : A -> Type) : forall {n}, vec n -> Type :=
+  | ForallT_nil : ForallT P (nil)
+  | ForallT_cons : forall n (x : A) (l : vec n), P x -> ForallT P l -> ForallT P (@cons A x n l).
 
-  Inductive vec_in {A : Type} (a : A) : forall {n}, vec A n -> Type :=
-  | vec_inB {n} (v : vec A n) : vec_in a (@cons A a n v)
-  | vec_inS a' {n} (v : vec A n) : vec_in a v -> vec_in a (@cons A a' n v).
+  Inductive vec_in {A : Set} (a : A) : forall {n}, vec n -> Type :=
+  | vec_inB {n} (v : vec n) : vec_in a (@cons _ a n v)
+  | vec_inS a' {n} (v : vec n) : vec_in a v -> vec_in a (@cons _ a' n v).
   Hint Constructors vec_in : core.
   
-  Lemma term_rect' (p : term -> Type) :
+  Lemma term_rect' (p : term -> Set) :
     (forall x, p (fvar x)) ->
     (forall x, p (bvar x)) -> 
     (forall F v, (ForallT p v) -> p (func F v)) -> forall (t : term), p t.
@@ -194,14 +179,14 @@ Section fix_signature.
       + econstructor. now eapply strong_term_ind'. eauto.
   Qed.
 
-  Lemma term_rect (p : term -> Type) :
+  Lemma term_rect (p : term -> Set) :
     (forall x, p (fvar x)) -> (forall x, p (bvar x)) -> (forall F v, (forall t, vec_in t v -> p t) -> p (func F v)) -> forall (t : term), p t.
   Proof.
     intros f1 f2 f3. eapply term_rect'.
     - apply f1.
     - apply f2.
-    - intros. apply f3. intros t. induction 1; inversion X; subst; eauto.
-      apply Eqdep_dec.inj_pair2_eq_dec in H2; subst; eauto. decide equality.
+    - intros F v H. apply f3. intros t. induction 1; inversion H; subst; eauto.
+      apply Eqdep_dec.inj_pair2_eq_dec in H3; subst; eauto. decide equality.
   Qed.
 
   Lemma term_ind (p : term -> Prop) :
@@ -210,91 +195,78 @@ Section fix_signature.
     intros f1 f2 f3. eapply term_rect'.
     - apply f1.
     - apply f2.
-    - intros. apply f3. intros t. induction 1; inversion X; subst; eauto.
+    - intros F v H. apply f3. intros t. induction 1; inversion H; subst; eauto.
       apply Eqdep_dec.inj_pair2_eq_dec in H3; subst; eauto. decide equality.
   Qed.
 
-  Inductive wf_term : term -> nat -> Prop :=
-  | wf_fvar x n : wf_term (fvar x) n
-  | wf_bvar x n : x < n -> wf_term (bvar x) n
-  | wf_funcs f v n :
-    Vector.Forall (fun t => wf_term t n) v
-  ->
-    wf_term (func f v) n
-  .
+  Fixpoint wf_term (t : term) (n : nat) : bool :=
+  match t with
+   | bvar x => x <? n
+   | fvar x => true
+   | func f x => fold_right (fun t Acc => andb Acc (wf_term t n)) x true
+  end.
 
-  Inductive wf_form : form -> nat -> Prop :=
-  | wf_fal n : wf_form fal n
-  | wf_pred P x n : 
-    Vector.Forall (fun t => wf_term t n) x
-  ->
-    wf_form (atom P x) n
-  | wf_impl f1 f2 n:
-    wf_form f1 n -> wf_form f2 n
-  ->
-    wf_form (impl f1 f2) n
-  | wf_exs f n :
-    wf_form f (S n)
-  ->
-    wf_form (exs f) n.
+  Fixpoint wf_form (F : form) (n : nat) : bool :=
+  match F with
+   | fal => true
+   | atom P x => fold_right (fun t Acc => andb Acc (wf_term t n)) x true
+   | impl x x0 => wf_form x n && wf_form x0 n
+   | exs x => wf_form x (S n)
+  end.
 
   Theorem wf_increase_term :
     forall t n, wf_term t n -> forall n', n' >= n -> wf_term t n'.
   Proof.
-    induction t; intros.
-    * constructor.
-    * constructor. inversion H. subst. lia.
-    * inversion H. subst. constructor; auto. simpl_existT. subst.
-      eapply Forall_impl_ext. 2: exact H4.
-      intros. simpl in H1. eapply IH. 2: simpl in H2; exact H2. auto. lia.
+    induction t; intros n H n' H0; auto.
+    * simpl in *. apply Nat.leb_le in H. apply Nat.leb_le. lia.
+    * simpl in *. induction v; auto; simpl.
+      simpl in H. do 2 separate.
+      erewrite IH. split; auto. apply IHv; auto.
+      - intros t H n1 H1 n'0 H2. eapply IH. now constructor. exact H1. auto.
+      - constructor.
+      - exact E2.
+      - auto.
   Qed.
 
   Theorem wf_increase :
     forall φ n, wf_form φ n -> forall n', n' >= n -> wf_form φ n'.
   Proof.
-    induction φ; intros.
-    * constructor.
-    * inversion H; subst. constructor; auto. simpl_existT. subst.
-      eapply Forall_impl. 2: exact H4.
-      intros. simpl in H1. eapply wf_increase_term. exact H1. auto.
-    * inversion H. subst. constructor. eapply IHφ1; eauto. eapply IHφ2; eauto.
-    * inversion H. subst. constructor. eapply IHφ; eauto. lia.
+    induction φ; intros n H n' H0; auto.
+    * simpl in *. induction v; auto; simpl.
+      simpl in H. do 2 separate.
+      erewrite wf_increase_term. split; auto. apply IHv; auto.
+      - eapply wf_increase_term. exact E2. auto.
+      - auto.
+    * simpl in *. apply andb_true_iff in H as [E1 E2].
+      erewrite IHφ1, IHφ2; [ auto | | | |]; eassumption.
+    * simpl in *. erewrite IHφ. 2: exact H. auto. lia.
   Qed.
 
   Theorem wf_term_subst :
     forall b t n, wf_term b (S n) -> wf_term t n ->
       wf_term (bsubst_term b t n) n.
   Proof.
-    induction b; intros; inversion H; subst.
+    induction b; intros t n H H0; inversion H; subst.
     * constructor.
     * simpl. break_match_goal.
-      - now constructor.
+      - simpl. now apply Nat.ltb_lt.
       - auto.
-      - lia.
-    * simpl. constructor. simpl_existT. subst.
-      eapply Forall_impl_ext in H4.
-      2: { intros. eapply IH. exact H1. exact H2. exact H0. }
-      clear H IH H0. induction v; simpl; constructor.
-      inversion H4; auto.
-      inversion H4; auto. simpl_existT. subst.
-      now apply IHv.
+      - simpl. apply Nat.ltb_lt in H2. lia.
+    * simpl in *; induction v; simpl in *; auto.
+      do 2 separate. rewrite IH; auto. constructor. split; auto.
+      apply IHv; auto. intros t0 H. apply IH. now constructor 2.
   Qed.
 
   Theorem wf_form_subst :
     forall φ t n, wf_form φ (S n) -> wf_term t n ->
       wf_form (bsubst_form φ t n) n.
   Proof.
-    induction φ; intros; simpl.
-    * constructor.
-    * inversion H. subst. constructor.
-      eapply Forall_impl_ext in H4.
-      2: { intros. eapply wf_term_subst. exact H2. exact H0. }
-      simpl_existT. subst.
-      clear H H0. induction v; simpl; constructor.
-      inversion H4; auto.
-      inversion H4; auto. simpl_existT. subst. now apply IHv.
-    * inversion H. subst. constructor. apply IHφ1; auto. apply IHφ2; auto.
-    * inversion H. subst. constructor. apply IHφ; auto. eapply wf_increase_term. exact H0.
+    induction φ; intros t n H H0; simpl; auto.
+    * simpl in *; induction v; simpl in *; auto. do 2 separate.
+      rewrite wf_term_subst; auto. split; auto.
+      apply IHv; auto.
+    * simpl in H. separate. rewrite IHφ1; auto. rewrite IHφ2; auto.
+    * simpl in H. subst. apply IHφ; auto. eapply wf_increase_term. exact H0.
       lia.
   Qed.
 
@@ -304,18 +276,19 @@ Section semantics.
   Context {Σ_vars : FOL_variables}.
   Context {Σ_funcs : funcs_signature}.
   Context {Σ_preds : preds_signature}.
-  Variable domain : Type.
+  Variable domain : Set.
 
   Class interp := B_I
     {
-      i_f : forall f : funs, vec domain (ar_funs f) -> domain ;
-      i_P : forall P : preds, vec domain (ar_preds P) -> bool ; (* for decidability *)
+      i_f : forall f : funs, @vec domain (ar_funs f) -> domain ;
+      i_P : forall P : preds, @vec domain (ar_preds P) -> bool ; (* for decidability *)
     }.
     Context {I : interp }.
     Definition env := vars -> domain. (* for free vars *)
     Variable failure : domain. (* for wrong evaluation!!! *)
 
-    Fixpoint mmap {A B : Type} (f : A -> option B) {n : nat} (v : t A n) : option (t B n) :=
+    Fixpoint mmap {A B : Type} (f : A -> option B) {n : nat} (v : t A n) : 
+      option (t B n) :=
     match v in (t _ n0) return (option (t B n0)) with
     | nil => Some nil
     | @cons _ a n0 v' => match f a with
@@ -328,13 +301,11 @@ Section semantics.
     end.
 
     Fixpoint eval (rho : env) (t : term) : domain :=
-      match t with
-      | fvar s => rho s
-      | bvar s => failure (* for wf terms, this is never used *)
-      | func f v => i_f f (Vector.map (eval rho) v)
-      end.
-
-    Print evar_open.
+    match t with
+    | fvar s => rho s
+    | bvar s => failure (* for wf terms, this is never used *)
+    | func f v => i_f f (Vector.map (eval rho) v)
+    end.
 
     Definition update_env (ρ : env) (x : vars) (d : domain) : env :=
       fun v => if var_eqdec v x then d else ρ v.
@@ -368,9 +339,9 @@ Section semantics.
     Theorem subst_var_size :
       forall f x y, form_size f = form_size (bsubst_form f (fvar x) y).
     Proof.
-      induction f; intros; auto; simpl.
-      - now rewrite (IHf1 x y), (IHf2 x y).
-      - now rewrite (IHf x (S y)).
+      induction f; intros x y; auto; simpl.
+      - now rewrite -> (IHf1 x y), -> (IHf2 x y).
+      - now rewrite -> (IHf x (S y)).
     Qed.
 
     Program Fixpoint sat (rho : env) (phi : form) {measure (form_size phi)} : Prop :=
@@ -394,30 +365,42 @@ Section semantics.
     Proposition sat_impl : forall ρ φ₁ φ₂, sat ρ (impl φ₁ φ₂) = 
                                             (sat ρ φ₁ -> sat ρ φ₂).
     Proof.
-      intros. unfold sat, sat_func.
+      intros ρ φ₁ φ₂. unfold sat, sat_func.
       rewrite fix_sub_eq.
-      Tactics.program_simpl. unfold projT1, projT2. intros.
-      destruct x, f0; auto.
-      rewrite H, H; auto.
-      f_equal. extensionality d. rewrite H. auto.
+      Tactics.program_simpl. unfold projT1, projT2.
+      destruct X; auto with f_equal.
+      { f_equal. apply propositional_extensionality.
+        epose proof (H _). epose proof (H _).
+        apply ZifyClasses.eq_iff in H0. apply ZifyClasses.eq_iff in H1. split; intros.
+        - eapply H0 in H2. exact H2. apply H1. auto.
+        - eapply H0 in H2. exact H2. apply H1. auto. 
+      }
+      { f_equal. apply functional_extensionality; auto. }
+      { f_equal. }
     Qed.
     Proposition sat_exs : forall ρ φ, sat ρ (exs φ) = 
                         (let x := var_fresh (form_vars φ) in
       exists d : domain, sat (update_env ρ x d) (bsubst_form φ (fvar x) 0)).
     Proof.
-      intros. unfold sat, sat_func.
+      intros ρ φ. unfold sat, sat_func.
       rewrite fix_sub_eq.
-      Tactics.program_simpl. unfold projT1, projT2. intros.
-      destruct x, f0; auto.
-      rewrite H, H; auto.
-      f_equal. extensionality d. rewrite H. auto.
+      Tactics.program_simpl. unfold projT1, projT2.
+      destruct X; auto with f_equal.
+      { f_equal. apply propositional_extensionality.
+        epose proof (H _). epose proof (H _).
+        apply ZifyClasses.eq_iff in H0. apply ZifyClasses.eq_iff in H1. split; intros.
+        - eapply H0 in H2. exact H2. apply H1. auto.
+        - eapply H0 in H2. exact H2. apply H1. auto. 
+      }
+      { f_equal. apply functional_extensionality; auto. }
+      { f_equal. }
     Qed.
 
     Notation "rho ⊨ phi" := (sat rho phi) (at level 20).
 
   Theorem sat_dec : forall φ ρ, {ρ ⊨ φ} + {~ ρ ⊨ φ}.
   Proof.
-    induction φ; intros.
+    induction φ; intros ρ.
     * right. auto.
     * rewrite sat_atom. apply bool_dec.
     * destruct (IHφ1 ρ), (IHφ2 ρ).
@@ -425,7 +408,7 @@ Section semantics.
       congruence.
       right. rewrite sat_impl. intros. auto.
     * rewrite sat_exs. admit. (* TODO: not trivial, maybe using size based induction *)
-  Admitted.
+  Abort.
 
 End semantics.
 
@@ -433,7 +416,6 @@ Section proof_system.
   Context {Σ_vars : FOL_variables}.
   Context {Σ_funcs : funcs_signature}.
   Context {Σ_preds : preds_signature}.
-  Print evar_quantify.
 
   Fixpoint quantify_term (t : term) (v : vars) (n : nat) : term :=
   match t with
@@ -453,7 +435,7 @@ Section proof_system.
 
 
   Reserved Notation "Γ ⊢_FOL form" (at level 50).
-  Inductive Hilbert_proof_sys (Γ : (list form)): form -> Prop :=
+  Inductive Hilbert_proof_sys (Γ : (list form)): form -> Set :=
   | AX (φ : form)             : wf_form φ 0 -> List.In φ Γ -> Γ ⊢_FOL φ
   | P1F (φ ψ : form)          : wf_form φ 0 -> wf_form ψ 0 -> Γ ⊢_FOL impl φ (impl ψ φ)
   | P2F (φ ψ ξ : form)        : wf_form φ 0 -> wf_form ψ 0 -> wf_form ξ 0 ->
@@ -480,33 +462,29 @@ Section soundness_completeness.
   Context {Σ_preds : preds_signature}.
   Notation "rho ⊨_FOL phi" := (sat _ _ _ rho phi) (at level 50).
   Notation "Γ ⊢_FOL form" := (Hilbert_proof_sys Γ form) (at level 50).
-  Check sat.
+
   Definition valid A phi :=
-    forall D (fail : D) (I : interp D) (rho : vars -> D),(forall Phi, List.In Phi A -> sat D fail rho Phi)
+    forall (D : Set) (fail : D) (I : interp D) (rho : vars -> D),(forall Phi, List.In Phi A -> sat D fail rho Phi)
       -> sat D fail rho phi.
 
   Theorem soundness :
     forall φ Γ, Γ ⊢_FOL φ -> valid Γ φ.
   Proof.
-    intros. induction H; subst; unfold valid; intros.
-    * now apply H1.
+    intros φ Γ H. induction H; subst; unfold valid; intros.
+    * now apply H.
     * do 2 rewrite sat_impl. intros. auto.
-    * repeat rewrite sat_impl. intros. apply H3; auto.
+    * repeat rewrite sat_impl. intros. apply H0; auto.
     * repeat rewrite sat_impl. intros.
-      destruct (sat_dec D fail φ rho); auto.
-      assert (~ sat D fail rho fal) by auto.
-      assert (sat D fail rho fal).
-      { apply H1. intros. congruence. }
-      congruence.
+      admit.
     * unfold valid in *.
-      apply IHHilbert_proof_sys1 in H3 as IH1.
-      apply IHHilbert_proof_sys2 in H3 as IH2. rewrite sat_impl in IH2. now apply IH2.
-    * rewrite sat_impl, sat_exs. intros.
+      apply IHHilbert_proof_sys1 in H1 as IH1.
+      apply IHHilbert_proof_sys2 in H1 as IH2. rewrite sat_impl in IH2. now apply IH2.
+    * rewrite -> sat_impl, -> sat_exs. intros.
       exists (eval D fail rho t).
       admit. (* TODO... *)
-    * rewrite sat_impl, sat_exs. intros. unfold valid in *.
-      apply IHHilbert_proof_sys in H3. rewrite sat_impl in H3. apply H3.
-      destruct H4. simpl in H4.
+    * rewrite -> sat_impl, -> sat_exs. intros. unfold valid in *.
+      apply IHHilbert_proof_sys in H0. rewrite sat_impl in H0. apply H0.
+      destruct H1. simpl in H1.
       remember (var_fresh (form_vars (quantify_form φ x 0))) as FF.
       admit. (* TODO... *)
   Admitted.
@@ -520,10 +498,11 @@ Section FOL_ML_correspondence.
   Context {Σ_funcs : funcs_signature}.
   Context {Σ_preds : preds_signature}.
 
-  Inductive Symbols :=
+  Inductive Symbols : Set :=
   | sym_fun   (name : funs)
   | sym_pred  (name : preds)
   | sym_import_definedness (d : Definedness.Symbols).
+
   Lemma Symbols_dec : forall (s1 s2 : Symbols), {s1 = s2} + {s1 <> s2}.
   Proof.
     repeat decide equality.
@@ -625,85 +604,80 @@ Section FOL_ML_correspondence.
   Notation "Γ ⊢_FOL form" := (Hilbert_proof_sys Γ form) (at level 50).
   Notation "Γ ⊢_ML form" := (ML_proof_system Γ form) (at level 50).
 
-  Theorem wf_term_FOL_ML : forall t n m,
-    wf_term t n -> is_true (well_formed_closed_aux (convert_term t) n m).
+  Theorem closed_term_FOL_ML : forall t n m,
+    wf_term t n -> well_formed_closed_aux (convert_term t) n m.
   Proof.
-    induction t using term_ind; intros.
-    * constructor.
-    * simpl. inversion H. now apply Nat.ltb_lt.
-    * simpl. inversion H. simpl_existT. subst. clear H. 
+    induction t; intros n m H; auto.
+    * simpl in *.
       remember (@patt_sym sig (sym_fun F)) as start.
       assert (is_true (well_formed_closed_aux start n m)). { rewrite Heqstart. auto. }
       clear Heqstart. generalize dependent start. induction v.
       - simpl. auto.
-      - simpl. inversion H3. simpl_existT. subst. intros.
-        epose proof (IHv _ H4 (start $ convert_term h)%ml). apply H0.
-        simpl. rewrite H, IH; auto. constructor.
-    Unshelve. intros. apply IH. now constructor 2. auto.
+      - intros start H0. simpl. simpl in H. separate.
+        apply IHv; auto.
+        intros t H1 n1 m0 H2. apply IH. now constructor 2. auto.
+        simpl. rewrite -> H0, -> IH; auto. constructor.
   Qed.
 
-  Theorem wf_aux_FOL_ML : forall φ n m,
-    wf_form φ n -> is_true (well_formed_closed_aux (convert_form φ) n m).
+  Theorem closed_form_FOL_ML : forall φ n m,
+    wf_form φ n -> well_formed_closed_aux (convert_form φ) n m.
   Proof.
-    induction φ; intros; auto.
-    * simpl. inversion H. simpl_existT. subst. clear H.
+    induction φ; intros n m H; simpl; auto.
+    * simpl in *.
       remember (@patt_sym sig (sym_pred P)) as start.
       assert (is_true (well_formed_closed_aux start n m)). { rewrite Heqstart. auto. }
       clear Heqstart. generalize dependent start. induction v.
       - simpl. auto.
-      - simpl. inversion H3. simpl_existT. subst. intros.
-        epose proof (IHv H4 (start $ convert_term h)%ml). apply H0.
-        simpl. rewrite H, wf_term_FOL_ML; auto.
-    * simpl. inversion H. subst. rewrite IHφ1, IHφ2; auto.
-    * simpl. inversion H. subst. rewrite IHφ; auto.
+      - simpl in *. separate. intros start H.
+        apply IHv; auto. simpl. rewrite -> closed_term_FOL_ML, -> H; auto.
+    * simpl in *. separate. subst. rewrite -> IHφ1, -> IHφ2; auto.
   Qed.
 
   Theorem positive_term_FOL_ML : forall t,
-    is_true (well_formed_positive (convert_term t)).
+    well_formed_positive (convert_term t).
   Proof.
-    induction t; intros; auto.
+    induction t; auto.
     * simpl. remember (@patt_sym sig (sym_fun F)) as start.
       assert (is_true (well_formed_positive start)) by now rewrite Heqstart.
-      clear Heqstart. generalize dependent start. induction v; intros; auto.
+      clear Heqstart. generalize dependent start.
+      induction v; intros start H; auto.
       simpl. apply IHv.
       - intros. apply IH; auto. now constructor 2.
-      - simpl. rewrite H, IH; auto. constructor.
+      - simpl. rewrite -> H, -> IH; auto. constructor.
   Qed.
 
   Theorem positive_form_FOL_ML : forall φ,
-    is_true (well_formed_positive (convert_form φ)).
+    well_formed_positive (convert_form φ).
   Proof.
-    induction φ; intros; auto.
+    induction φ; auto.
     * simpl. remember (@patt_sym sig (sym_pred P)) as start.
       assert (is_true (well_formed_positive start)) by now rewrite Heqstart.
-      clear Heqstart. generalize dependent start. induction v; intros; auto.
+      clear Heqstart. generalize dependent start. induction v; intros start H; auto.
       simpl. apply IHv.
-      simpl. rewrite H, positive_term_FOL_ML; auto.
-    * simpl. rewrite IHφ1, IHφ2; auto.
+      simpl. rewrite -> H, -> positive_term_FOL_ML; auto.
+    * simpl. rewrite -> IHφ1, -> IHφ2; auto.
   Qed.
 
-  Corollary wf_FOL_ML_term : forall t,
-    wf_term t 0 -> is_true (well_formed (convert_term t)).
+  Corollary wf_term_FOL_ML : forall t,
+    wf_term t 0 -> well_formed (convert_term t).
   Proof.
-    intros. unfold well_formed. unfold is_true.
-    apply andb_true_intro. split.
+    intros t H. unfold well_formed. separate. split.
     * apply positive_term_FOL_ML.
-    * now apply wf_term_FOL_ML.
+    * now apply closed_term_FOL_ML.
   Qed.
 
-  Corollary wf_FOL_ML : forall φ,
-    wf_form φ 0 -> is_true (well_formed (convert_form φ)).
+  Corollary wf_form_FOL_ML : forall φ,
+    wf_form φ 0 -> well_formed (convert_form φ).
   Proof.
-    intros. unfold well_formed. unfold is_true.
-    apply andb_true_intro. split.
+    intros φ H. unfold well_formed. separate. split.
     * apply positive_form_FOL_ML.
-    * now apply wf_aux_FOL_ML.
+    * now apply closed_form_FOL_ML.
   Qed.
 
-  Theorem in_theory : forall Γ x,
+  Theorem in_FOL_theory : forall Γ x,
     List.In x Γ -> Ensembles.In _ (from_FOL_theory Γ) (convert_form x).
   Proof.
-    induction Γ; intros.
+    induction Γ; intros x H.
     * inversion H.
     * simpl. inversion H.
       - apply Ensembles.Union_introl. subst. apply Ensembles.In_singleton.
@@ -711,88 +685,22 @@ Section FOL_ML_correspondence.
         now apply Ensembles.Union_intror.
   Qed.
 
-  Hint Resolve wf_FOL_ML : core.
-  Print exists_quantify.
-  Print evar_quantify.
-  Print quantify_form.
+  Hint Resolve wf_form_FOL_ML : core.
+  Hint Resolve wf_term_FOL_ML : core.
 
-  (** TO ML *)
-  Theorem double_evar_quantify φ : forall x n,
-    evar_quantify x n (evar_quantify x n φ) = evar_quantify x n φ.
-  Proof.
-    induction φ; intros; simpl; auto.
-    * break_match_goal; simpl; auto. rewrite Heqb. auto.
-    * now rewrite IHφ1, IHφ2.
-    * now rewrite IHφ1, IHφ2.
-    * now rewrite IHφ.
-    * now rewrite IHφ.
-  Qed.
-
-  (** TO ML *)
-  Lemma bevar_subst_identity φ : forall ψ n k m,
-    m >= n -> is_true (well_formed_closed_aux φ n k)
-  ->
-    bevar_subst φ ψ m = φ.
-  Proof.
-    induction φ; intros; simpl; auto.
-    * simpl in H0. break_match_goal; auto. apply NPeano.Nat.ltb_lt in H0. lia.
-    * simpl in H0. apply eq_sym, andb_true_eq in H0. destruct H0. erewrite IHφ1, IHφ2.
-      3: apply eq_sym, H1.
-      4: apply eq_sym, H0. all: auto.
-    * simpl in H0. apply eq_sym, andb_true_eq in H0. destruct H0. erewrite IHφ1, IHφ2.
-      3: apply eq_sym, H1.
-      4: apply eq_sym, H0. all: auto.
-    * simpl in H0. erewrite IHφ. 3: apply H0. auto. lia.
-    * simpl in H0. erewrite IHφ. 3: apply H0. all: auto.
-  Qed.
-
-  (** TO ML *)
-  Lemma well_formed_aux_increase φ: forall n m n' m', n' >= n -> m' >= m ->
-    is_true (well_formed_closed_aux φ n m) ->
-    is_true (well_formed_closed_aux φ n' m').
-  Proof.
-    induction φ; intros; simpl; auto.
-    * simpl in H1. apply NPeano.Nat.ltb_lt in H1. apply NPeano.Nat.ltb_lt. lia.
-    * simpl in H1. apply NPeano.Nat.ltb_lt in H1. apply NPeano.Nat.ltb_lt. lia.
-    * simpl in H1. apply eq_sym, andb_true_eq in H1. destruct H1.
-      erewrite IHφ1, IHφ2. auto. 3: apply eq_sym, H2. 5: apply eq_sym, H1.
-      all: lia.
-    * simpl in H1. apply eq_sym, andb_true_eq in H1. destruct H1.
-      erewrite IHφ1, IHφ2. auto. 3: apply eq_sym, H2. 5: apply eq_sym, H1.
-      all: lia.
-    * simpl in H1. erewrite IHφ. 4: exact H1. all: auto; lia.
-    * simpl in H1. erewrite IHφ. 4: exact H1. all: auto; lia.
-  Qed.
-
-  (** TO ML *)
-  Theorem double_evar_bevar_subst φ : forall ψ n k,
-    is_true (well_formed_closed_aux ψ n k) ->
-    bevar_subst (bevar_subst φ ψ n) ψ n = bevar_subst φ ψ n.
-  Proof.
-    induction φ; intros; simpl; auto.
-    * break_match_goal; simpl; auto.
-      - rewrite Heqc. auto.
-      - erewrite bevar_subst_identity. 3: exact H. all: auto. 
-      - rewrite Heqc. auto.
-    * erewrite IHφ1, IHφ2; eauto.
-    * erewrite IHφ1, IHφ2; eauto.
-    * erewrite IHφ. auto. eapply well_formed_aux_increase. 3: exact H. lia. auto.
-    * erewrite IHφ. auto. eapply well_formed_aux_increase. 3: exact H. lia. auto.
-  Qed.
-
-  Lemma pointwise_fold : forall n0 (v : vec term n0) start (F : Pattern -> Pattern),
+  Lemma pointwise_fold : forall n0 (v : @vec term n0) start (F : Pattern -> Pattern),
     (forall (p1 p2 : Pattern), F (patt_app p1 p2) = patt_app (F p1) (F p2)) ->
     F (fold_left (λ (Acc : Pattern) (t : term), (Acc $ convert_term t)%ml)
      start v) =
   (fold_left (λ (Acc : Pattern) (t : term), (Acc $ F (convert_term t))%ml)
      (F start) v).
   Proof.
-    induction v; intros.
+    induction v; intros start F H.
     * simpl. auto.
-    * simpl. rewrite IHv, H. auto. apply H.
+    * simpl. rewrite -> IHv, -> H. auto. apply H.
   Qed.
 
-  Corollary evar_quantify_fold : forall n0 (v : vec term n0) start x n,
+  Corollary evar_quantify_fold : forall n0 (v : @vec term n0) start x n,
     evar_quantify x n (fold_left (λ (Acc : Pattern) (t : term), (Acc $ convert_term t)%ml)
      start v) =
   (fold_left (λ (Acc : Pattern) (t : term), (Acc $ evar_quantify x n (convert_term t))%ml)
@@ -802,7 +710,7 @@ Section FOL_ML_correspondence.
   Qed.
 
   (** This is boiler-plate *)
-  Corollary bevar_subst_fold : forall n0 (v : vec term n0) start x n,
+  Corollary bevar_subst_fold : forall n0 (v : @vec term n0) start x n,
     bevar_subst (fold_left (λ (Acc : Pattern) (t : term), (Acc $ convert_term t)%ml)
      start v) x n =
   (fold_left (λ (Acc : Pattern) (t : term), (Acc $ bevar_subst (convert_term t) x n)%ml)
@@ -817,48 +725,50 @@ Section FOL_ML_correspondence.
     forall t n x, convert_term (quantify_term t x n) = 
                   evar_quantify x n (convert_term t).
   Proof.
-    induction t; intros; auto; cbn.
-    * now destruct (var_eqdec x0 x).
+    induction t; intros n x'; auto; cbn.
+    * now destruct (var_eqdec x' x).
     * remember (@patt_sym sig (sym_fun F)) as start.
       rewrite fold_left_map.
-      assert (start = evar_quantify x n start) by now rewrite Heqstart.
+      assert (start = evar_quantify x' n start) by now rewrite Heqstart.
       clear Heqstart.
       generalize dependent start.
       induction v; intros; simpl; auto.
-      rewrite IHv. do 2 rewrite evar_quantify_fold.
-      simpl. rewrite IH, double_evar_quantify. auto.
-      - constructor.
-      - intros. apply IH. constructor 2; auto.
+      rewrite IHv.
+      - intros. apply IH. now constructor 2.
       - simpl. rewrite <- H, IH, double_evar_quantify; auto. constructor.
+      - do 2 rewrite evar_quantify_fold.
+        simpl. rewrite -> IH, -> double_evar_quantify. auto. simpl.
+        constructor.
   Qed.
 
   Theorem quantify_form_correspondence :
     forall φ n x, convert_form (quantify_form φ x n) = 
                   evar_quantify x n (convert_form φ).
   Proof.
-    induction φ; intros; auto; cbn.
+    induction φ; intros n x'; auto; cbn.
     * remember (@patt_sym sig (sym_pred P)) as start.
       rewrite fold_left_map.
-      assert (start = evar_quantify x n start) by now rewrite Heqstart.
+      assert (start = evar_quantify x' n start) by now rewrite Heqstart.
       clear Heqstart.
       generalize dependent start.
       induction v; intros; simpl; auto.
-      rewrite IHv. do 2 rewrite evar_quantify_fold.
-      simpl. rewrite quantify_term_correspondence, double_evar_quantify. auto.
+      rewrite IHv.
       - simpl. rewrite <- H, quantify_term_correspondence, double_evar_quantify; auto.
-    * now rewrite IHφ1, IHφ2.
+      - do 2 rewrite evar_quantify_fold.
+        simpl. rewrite -> quantify_term_correspondence, -> double_evar_quantify. auto.
+    * now rewrite -> IHφ1, -> IHφ2.
     * now rewrite IHφ.
   Qed.
 
   Theorem term_vars_free_vars_notin :
     forall t x, ~List.In x (term_vars t) -> x ∉ (free_evars (convert_term t)).
   Proof.
-    induction t using term_ind; intros.
-    * simpl. intro. apply H. simpl. apply sets.elem_of_singleton_1 in H0. auto.
+    induction t; intros x' H.
+    * simpl. intros H0. apply H. simpl. apply sets.elem_of_singleton_1 in H0. auto.
     * intro. simpl in H0. inversion H0.
     * simpl in H. simpl. 
       remember (@patt_sym sig (sym_fun F)) as start.
-      assert (x ∉ free_evars start) by now rewrite Heqstart.
+      assert (x' ∉ free_evars start) by now rewrite Heqstart.
       clear Heqstart. generalize dependent start. 
       induction v; intros.
       - auto.
@@ -875,11 +785,11 @@ Section FOL_ML_correspondence.
   Theorem form_vars_free_vars_notin :
     forall φ x, ~List.In x (form_vars φ) -> x ∉ (free_evars (convert_form φ)).
   Proof.
-    induction φ; intros; auto.
+    induction φ; intros x' H; auto.
     * intro. inversion H0.
     * simpl in H. simpl. 
       remember (@patt_sym sig (sym_pred P)) as start.
-      assert (x ∉ free_evars start) by now rewrite Heqstart.
+      assert (x' ∉ free_evars start) by now rewrite Heqstart.
       clear Heqstart. generalize dependent start. 
       induction v; intros.
       - auto.
@@ -899,7 +809,7 @@ Section FOL_ML_correspondence.
                   convert_term (bsubst_term b t n) = 
                   bevar_subst (convert_term b) (convert_term t) n.
   Proof.
-    induction b; intros; auto.
+    induction b; intros t n H; auto.
     * simpl. now break_match_goal.
     * simpl. remember (@patt_sym sig (sym_fun F)) as start.
       rewrite fold_left_map.
@@ -907,15 +817,13 @@ Section FOL_ML_correspondence.
       clear Heqstart.
       generalize dependent start.
       induction v; intros; simpl; auto.
-      rewrite IHv. do 2 rewrite bevar_subst_fold.
-      simpl. erewrite IH, double_evar_bevar_subst. auto.
-      - apply wf_term_FOL_ML. apply H.
-      - constructor.
-      - intros. apply H.
+      rewrite IHv. 
       - intros. apply IH. constructor 2; auto. auto.
-      - simpl. erewrite <- H0, IH, double_evar_bevar_subst; auto.
-        apply wf_term_FOL_ML. auto.
-        constructor.
+      - simpl. erewrite <- H0, IH, double_bevar_subst; auto.
+        apply closed_term_FOL_ML. auto. constructor.
+      - do 2 rewrite bevar_subst_fold.
+        simpl. erewrite IH, double_bevar_subst; auto.
+        apply closed_term_FOL_ML. auto. constructor.
     Unshelve. all: exact 0.
   Qed.
 
@@ -924,7 +832,7 @@ Section FOL_ML_correspondence.
                   convert_form (bsubst_form φ t n) = 
                   bevar_subst (convert_form φ) (convert_term t) n.
   Proof.
-    induction φ; intros; auto.
+    induction φ; intros t n H; auto.
     * simpl.
       remember (@patt_sym sig (sym_pred P)) as start.
       rewrite fold_left_map.
@@ -932,127 +840,23 @@ Section FOL_ML_correspondence.
       clear Heqstart. revert H.
       generalize dependent start.
       induction v; intros; simpl; auto.
-      rewrite IHv. do 2 rewrite bevar_subst_fold.
-      simpl. erewrite bevar_subst_corr_term, double_evar_bevar_subst. auto.
-      - apply wf_term_FOL_ML. auto.
-      - auto.
+      rewrite IHv.
       - intros. rewrite bevar_subst_corr_term; auto.
-        simpl. erewrite double_evar_bevar_subst. rewrite <- H0. auto.
-        apply wf_term_FOL_ML. auto.
+        simpl. erewrite double_bevar_subst. rewrite <- H0. auto.
+        apply closed_term_FOL_ML. auto.
       - auto.
-    * simpl. now rewrite IHφ1, IHφ2.
-    * simpl. rewrite IHφ. auto. eapply wf_increase_term. apply H. lia.
+      - do 2 rewrite bevar_subst_fold.
+        simpl. erewrite bevar_subst_corr_term, double_bevar_subst. auto.
+        apply closed_term_FOL_ML; auto. auto.
+    * simpl. now rewrite -> IHφ1, -> IHφ2.
+    * simpl. rewrite IHφ. auto. eapply wf_increase_term. apply H. lia. auto.
     Unshelve. all: exact 0.
   Qed.
-
-  (*******************************************************)
-  (** TO ML *)
-  (* This has to go to FOL helpers *)
-  Lemma conj_intro_meta_partial :
-  ∀ (Γ : Theory) (A B : Pattern),
-    is_true (well_formed A) → is_true (well_formed B) → Γ ⊢_ML A → Γ ⊢_ML patt_imp B (patt_and A B).
-  Proof.
-    intros.
-    eapply (Modus_ponens _ _ _ _ _).
-    - exact H1.
-    - apply conj_intro; auto.
-    Unshelve. all: auto.
-  Qed.
-
-  Lemma and_impl_patt :
-    forall (A B C : Pattern) Γ, is_true (well_formed A) → is_true (well_formed B) → is_true (well_formed C) →
-    Γ ⊢_ML A -> Γ ⊢_ML ((A and B) ---> C) -> Γ ⊢_ML (B ---> C).
-  Proof.
-    intros.
-    Search patt_imp. Check syllogism_intro.
-    eapply syllogism_intro with (B0 := patt_and A B); auto.
-    apply conj_intro_meta_partial; auto.
-  Qed.
-
-  Lemma conj_intro2 (Γ : Theory) (A B : Pattern) :
-    is_true (well_formed A) -> is_true (well_formed B) -> Γ ⊢_ML (A ---> (B ---> (B and A))).
-  Proof.
-    intros. eapply reorder_meta; auto.
-    apply conj_intro; auto.
-  Qed.
-
-  Lemma conj_intro_meta_partial2 :
-  ∀ (Γ : Theory) (A B : Pattern),
-    is_true (well_formed A) → is_true (well_formed B) → Γ ⊢_ML A → Γ ⊢_ML patt_imp B (patt_and B A).
-  Proof.
-    intros.
-    eapply (Modus_ponens _ _ _ _ _).
-    - exact H1.
-    - Search patt_and. apply conj_intro2; auto.
-    Unshelve. all: auto.
-  Qed.
-
-  Lemma and_impl_patt2 :
-    forall (A B C : Pattern) Γ, is_true (well_formed A) → is_true (well_formed B) → is_true (well_formed C) →
-    Γ ⊢_ML A -> Γ ⊢_ML (patt_imp (patt_and B A) C) -> Γ ⊢_ML (patt_imp B C).
-  Proof.
-    intros.
-    Search patt_imp. Check syllogism_intro.
-    eapply syllogism_intro with (B0 := patt_and B A); auto.
-    pose conj_intro_meta_partial2; auto.
-  Qed.
-
-  Lemma patt_and_comm :
-    forall (A B : Pattern) Γ, is_true (well_formed A) → is_true (well_formed B)
-  ->
-    Γ ⊢_ML patt_and A B -> Γ ⊢_ML patt_and B A.
-  Proof.
-    intros.
-    apply pf_conj_elim_r_meta in H1 as P1.
-    apply pf_conj_elim_l_meta in H1 as P2. all: auto.
-    apply conj_intro_meta; auto.
-  Qed.
-
-  Lemma patt_iff_implies_equal :
-    forall φ1 φ2 Γ, is_true (well_formed φ1) -> is_true (well_formed φ2) ->
-    Γ ⊢_ML (φ1 <---> φ2) -> Γ ⊢_ML (patt_equal φ1 φ2).
-  Proof.
-    intros. Print Application_context. Check A_implies_not_not_A_ctx. Print patt_total.
-    epose proof (A_implies_not_not_A_ctx Γ (φ1 <---> φ2) (ctx_app_r box _)). 
-    apply H2; auto. unfold patt_iff, patt_and, patt_or, patt_not.
-    unfold well_formed, well_formed_closed in *.
-    apply andb_true_iff in H. apply andb_true_iff in H0. destruct H, H0. cbn.
-    now rewrite H, H0, H3, H4.
-    Unshelve.
-    auto.
-  Qed.
-
-  Lemma patt_equal_refl :
-    forall φ Γ, is_true (well_formed φ) ->
-    Γ ⊢_ML patt_equal φ φ.
-  Proof.
-    intros. pose proof (pf_iff_equiv_refl Γ φ H).
-    apply patt_iff_implies_equal in H0; auto.
-  Qed.
-
-  (*******************************************************)
-
-  (* Most important lemmas: *)
-  (** TO ML *)
-  Lemma exists_functional_subst :
-    forall φ φ' Γ, 
-      Γ ⊢_ML patt_imp (patt_and (instantiate (patt_exists φ) φ') (patt_exists (patt_equal φ' (patt_bound_evar 0)))) (patt_exists φ).
-  Proof.
-  
-  Admitted.
-
-  (** TO ML *)
-  Lemma forall_functional_subst :
-    forall φ φ' Γ, 
-      Γ ⊢_ML patt_imp (patt_and (patt_forall φ) (patt_exists (patt_equal φ' (patt_bound_evar 0)))) (bevar_subst φ φ' 0).
-  Proof.
-  
-  Admitted.
 
   Theorem ax_in :
     forall Γ F, Ensembles.In _ (from_FOL_theory Γ) (axiom F).
   Proof.
-    induction Γ; intros.
+    induction Γ; intros F.
     * simpl. unfold base_FOL_theory. econstructor.
       reflexivity.
     * simpl. apply Ensembles.Union_intror. apply IHΓ.
@@ -1063,7 +867,7 @@ Section FOL_ML_correspondence.
   Proof.
     induction n; intros.
     * cbn. auto.
-    * simpl. rewrite IHn, Nat.add_succ_comm. auto.
+    * simpl. rewrite -> IHn, -> Nat.add_succ_comm. auto.
   Qed.
 
   Lemma subst_make_list : forall n m ψ start, m > n ->
@@ -1079,89 +883,36 @@ Section FOL_ML_correspondence.
           (make_list1 n) (bevar_subst start ψ m)).
   Proof.
     induction n; intros; cbn; auto.
-    rewrite IHn. 2: lia. cbn. break_match_goal.
+    rewrite IHn. lia. cbn. break_match_goal.
     * congruence.
     * lia.
     * auto.
   Qed.
 
-  (** these lemmas should go to the other wf lemmas in ML *)
-  (** TO ML *)
-  Inductive mu_free : Pattern -> Prop :=
-  | free_evar_mu_free x : mu_free (patt_free_evar x)
-  | free_svar_mu_free x : mu_free (patt_free_svar x)
-  | bound_evar_mu_free x : mu_free (patt_bound_evar x)
-  | bound_svar_mu_free x : mu_free (patt_bound_svar x)
-  | sym_mu_free x : mu_free (patt_sym x)
-  | bott_mu_free : mu_free (patt_bott)
-  | app_mu_free p1 p2 : 
-    mu_free p1 -> mu_free p2
-   ->
-    mu_free (patt_app p1 p2)
-  | imp_mu_free p1 p2 : 
-    mu_free p1 -> mu_free p2
-   ->
-    mu_free (patt_imp p1 p2)
-  | exs_mu_free p :
-    mu_free p
-   ->
-    mu_free (patt_exists p)
-  .
-
   Lemma term_mu_free :
     forall t, mu_free (convert_term t).
   Proof.
-    induction t.
-    1-2: constructor.
+    induction t; auto.
     simpl. remember (@patt_sym sig (sym_fun F)) as start.
-    assert (mu_free start) by (rewrite Heqstart; constructor). clear Heqstart.
+    assert (is_true (mu_free start)) by (rewrite Heqstart; constructor). clear Heqstart.
     generalize dependent start.
     induction v; simpl.
-    * auto.
+    * intros. auto.
     * intros. eapply IHv.
-      intros. apply IH. constructor 2; auto. constructor. auto. apply IH. constructor.
+      intros. apply IH. constructor 2; auto.
+      simpl. rewrite H. auto. apply IH. constructor.
   Qed.
 
-  (** TO ML *)
-  Lemma well_formed_positive_bevar_subst φ : forall n ψ,
-    mu_free φ ->
-    is_true (well_formed_positive φ) -> is_true (well_formed_positive ψ)
-  ->
-    is_true (well_formed_positive (bevar_subst φ ψ n)).
+  Lemma form_mu_free:
+    forall φ, mu_free (convert_form φ).
   Proof.
-    induction φ; intros; simpl; auto.
-    2-3: inversion H; subst;
-         simpl in H0; apply eq_sym, andb_true_eq in H0; destruct H0; 
-         rewrite IHφ1, IHφ2; auto.
-    * break_match_goal; auto.
-    * inversion H. subst. rewrite IHφ; auto.
-    * inversion H.
-  Qed.
-
-  (** TO ML *)
-  Lemma well_formed_aux_bevar_subst φ : forall n m ψ,
-    is_true (well_formed_closed_aux φ (S n) m) -> is_true (well_formed_closed_aux ψ n m)
-  ->
-    is_true (well_formed_closed_aux (bevar_subst φ ψ n) n m).
-  Proof.
-    induction φ; intros; simpl; auto.
-    * break_match_goal; auto. simpl in H. simpl. apply NPeano.Nat.ltb_lt. auto.
-      simpl in H. apply NPeano.Nat.ltb_lt in H. lia.
-    * simpl in H. apply eq_sym, andb_true_eq in H. destruct H. rewrite IHφ1, IHφ2; auto.
-    * simpl in H. apply eq_sym, andb_true_eq in H. destruct H. rewrite IHφ1, IHφ2; auto.
-    * simpl. rewrite IHφ; auto.
-      eapply well_formed_aux_increase. 3: exact H0. all: lia.
-    * simpl. simpl in H. rewrite IHφ; auto.
-      eapply well_formed_aux_increase. 3: exact H0. all: lia.
-  Qed.
-
-  (** TO ML *)
-  Lemma well_formed_closed_all φ : forall n m,
-    is_true (well_formed_closed_aux (all , φ) n m)
-  <->
-    is_true (well_formed_closed_aux φ (S n) m).
-  Proof.
-    intros. simpl. do 2 rewrite andb_true_r. auto.
+    induction φ; auto.
+    * simpl. remember (@patt_sym sig (sym_pred P)) as start.
+      assert (is_true (mu_free start)) by (rewrite Heqstart; constructor). clear Heqstart.
+      generalize dependent start. induction v; simpl; auto.
+      intros start H. eapply IHv.
+      simpl. now rewrite -> H, -> term_mu_free.
+    * simpl. now rewrite -> IHφ1, -> IHφ2.
   Qed.
 
   Lemma well_formed_closed_prefix φ : forall n k m,
@@ -1170,16 +921,7 @@ Section FOL_ML_correspondence.
   Proof.
     induction n; simpl; auto; intros.
     do 2 rewrite andb_true_r.
-    rewrite IHn, NPeano.Nat.add_succ_r. auto.
-  Qed.
-
-  (** TO ML *)
-  Lemma well_formed_positive_all φ : 
-    is_true (well_formed_positive (all , φ))
-  <->
-    is_true (well_formed_positive φ).
-  Proof.
-    intros. simpl. do 2 rewrite andb_true_r. auto.
+    rewrite -> IHn, -> NPeano.Nat.add_succ_r. auto.
   Qed.
 
   Lemma well_formed_positive_prefix φ : forall n,
@@ -1198,7 +940,7 @@ Section FOL_ML_correspondence.
         (make_list1 n) start )
      m k).
   Proof.
-    induction n; intros; simpl; auto.
+    induction n; intros start m k H H0; simpl; auto.
     apply (IHn). lia. simpl. rewrite H0. simpl. apply NPeano.Nat.ltb_lt. lia.
   Qed.
 
@@ -1221,7 +963,7 @@ Section FOL_ML_correspondence.
         (make_list0 n) start)
      m k).
   Proof.
-    induction n; intros; simpl; auto.
+    induction n; intros start m k H H0; simpl; auto.
     apply (IHn). lia. simpl. rewrite H0. simpl. apply NPeano.Nat.ltb_lt. lia.
   Qed.
 
@@ -1232,55 +974,54 @@ Section FOL_ML_correspondence.
         (λ (Acc : Pattern) (x : nat), (Acc $ patt_bound_evar x)%ml)
         (make_list0 n) start)).
   Proof.
-    induction n; intros; simpl; auto.
+    induction n; intros start H; simpl; auto.
     apply (IHn). simpl. rewrite H. auto.
   Qed.
 
   Theorem ax_wf :
     forall F, is_true (well_formed (axiom F)).
   Proof.
-    unfold axiom. intros.
+    unfold axiom. intros F.
     break_match_goal.
     * unfold Definedness.axiom. destruct name. simpl. constructor.
     * unfold well_formed, well_formed_closed. apply andb_true_intro. split.
       - apply well_formed_positive_prefix. simpl. rewrite well_formed_positive_list. auto.
         auto.
       - apply well_formed_closed_prefix. simpl. rewrite well_formed_closed_list.
-        simpl. auto. lia. simpl. auto.
+        simpl. auto. lia. all: now simpl.
     * unfold well_formed, well_formed_closed. apply andb_true_intro. split.
       - apply well_formed_positive_prefix. simpl. rewrite well_formed_positive_list0. auto.
         auto.
       - apply well_formed_closed_prefix. simpl. rewrite well_formed_closed_list0.
-        simpl. auto. lia. simpl. auto.
+        simpl. auto. lia. all: now simpl.
   Qed.
 
   Proposition term_functionality :
     forall t Γ, wf_term t 0 ->
       from_FOL_theory Γ ⊢_ML patt_exists (patt_equal (convert_term t) (patt_bound_evar 0)).
   Proof.
-    induction t; intros.
+    induction t using term_rect; intros.
     * simpl.
       pose proof (Ex_quan (from_FOL_theory Γ ) (patt_equal (patt_free_evar x) (patt_bound_evar 0)) x).
       simpl in H0. eapply Modus_ponens. 4: exact H0.
       all: auto.
-      apply patt_equal_refl. constructor.
-    * inversion H. inversion H1.
+      epose proof (@patt_equal_refl _ _ (patt_free_evar x) (from_FOL_theory Γ) _).
+      exact H1.
+    * simpl in H. apply Nat.ltb_lt in H. lia.
     * assert (from_FOL_theory Γ ⊢_ML axiom (AxFun F)). {
         apply hypothesis. apply ax_wf. apply ax_in.
-      } simpl in H0.
+      } simpl in H1, H0.
       simpl. remember (@patt_sym sig (sym_fun F)) as start.
       assert (forall n ψ, bevar_subst start ψ n = start) as HIND. 
         { intros. rewrite Heqstart. auto. }
-      assert (mu_free start) as HMUF. { rewrite Heqstart. constructor. }
+      assert (is_true (mu_free start)) as HMUF. { rewrite Heqstart. constructor. }
       assert (is_true (well_formed start)) as WFS. { rewrite Heqstart. auto. }
       clear Heqstart. generalize dependent start.
-      assert (Forall (λ t : term, wf_term t 0) v). {
-        inversion H. simpl_existT. now subst.
-      } revert H0. clear H. induction v; intros.
+      revert H0. induction v; intros.
       - cbn. simpl in H1. exact H1.
       - cbn in *. eapply (IHv _ _ (start $ convert_term h)%ml).
-        clear IHv. inversion H0. simpl_existT. subst.
-        specialize (IH h ltac:(constructor) Γ H4).
+        clear IHv. separate.
+        specialize (H h ltac:(constructor) Γ E2).
         remember (add_forall_prefix n
             (ex ,
              patt_equal
@@ -1288,17 +1029,16 @@ Section FOL_ML_correspondence.
                   (λ (Acc : Pattern) (x : nat), (Acc $ patt_bound_evar x)%ml)
                   (make_list1 n) (start $ patt_bound_evar (S n))%ml)
                BoundVarSugar.b0)) as A.
-        pose proof (forall_functional_subst A (convert_term h) (from_FOL_theory Γ)).
+        pose proof (@forall_functional_subst _ _ A (convert_term h) (from_FOL_theory Γ)).
         assert (mu_free A). {
-          rewrite HeqA. clear H H5 H4 HIND H1 HeqA IH H0 h v Γ A F WFS.
+          rewrite HeqA. clear H HIND H1 HeqA E1 E2 H0 h v Γ A F WFS.
           generalize dependent start. induction n; simpl.
-          * repeat constructor. all: apply HMUF.
-          * do 3 constructor. apply IHn; constructor; auto. constructor.
-            constructor.
+          * intros. repeat constructor. all: rewrite HMUF; auto.
+          * intros. simpl. rewrite IHn; auto. simpl. now rewrite HMUF.
         }
-        assert (is_true (well_formed (all , A))) as WfA.
+        assert (well_formed (all , A)) as WfA.
         {
-          rewrite HeqA. clear H H5 H4 HIND H1 IH H0 h v Γ H2 HeqA A F HMUF.
+          rewrite HeqA. clear H E1 E2 H2 HIND H1 H H0 h v Γ H2 HeqA A F HMUF.
           unfold well_formed, well_formed_closed.
           apply eq_sym, andb_true_eq in WFS. destruct WFS.
           apply andb_true_intro. split.
@@ -1312,39 +1052,40 @@ Section FOL_ML_correspondence.
             repeat rewrite andb_true_r. rewrite well_formed_closed_list; auto.
             lia. simpl. apply andb_true_intro.
             split.
-            - eapply well_formed_aux_increase. 3: apply eq_sym, H0. all: lia.
+            - eapply wfc_aux_extend. apply eq_sym, H0. all: lia.
             - apply NPeano.Nat.ltb_lt. lia.
         }
         assert (from_FOL_theory Γ ⊢_ML (all , A and ex , patt_equal (convert_term h) BoundVarSugar.b0 )). {
           apply conj_intro_meta; auto.
           unfold well_formed. simpl. rewrite positive_term_FOL_ML.
-          unfold well_formed_closed. simpl. eapply wf_increase_term in H4.
-          eapply wf_term_FOL_ML in H4.
-          rewrite H4. auto. lia.
+          unfold well_formed_closed. simpl. apply wf_increase_term with (n' := 1) in E2. 2: lia.
+          eapply closed_term_FOL_ML in E2.
+          rewrite E2. auto.
         }
-        apply Modus_ponens in H; auto.
+        apply Modus_ponens in H0; auto.
         2: {
           unfold well_formed in *. simpl. rewrite positive_term_FOL_ML.
-          unfold well_formed_closed in *. simpl. eapply wf_increase_term in H4.
-          eapply wf_term_FOL_ML in H4.
-          rewrite H4. apply eq_sym, andb_true_eq in WfA. destruct WfA.
-          simpl in H7, H6. do 2 rewrite andb_true_r in H6, H7.
-          rewrite <- H7, <- H6. auto. lia.
+          unfold well_formed_closed in *. simpl. apply wf_increase_term with (n' := 1) in E2. 2: lia.
+          eapply closed_term_FOL_ML in E2.
+          rewrite E2. separate.
+          simpl in E0, E3. do 4 rewrite andb_true_r in E0, E3.
+          rewrite -> E0, -> E3. auto.
         }
         2: {
           unfold well_formed in *. simpl. rewrite positive_term_FOL_ML.
-          unfold well_formed_closed in *. simpl. eapply wf_increase_term in H4 as H4'.
-          eapply wf_term_FOL_ML in H4'.
-          rewrite H4'. apply eq_sym, andb_true_eq in WfA. destruct WfA.
-          simpl in H7, H6. do 2 rewrite andb_true_r in H7, H6.
-          rewrite <- H7, <- H6. auto.
-          rewrite well_formed_positive_bevar_subst; auto.
-          2: apply positive_term_FOL_ML. 2: lia. simpl.
-          apply well_formed_aux_bevar_subst; auto. apply wf_term_FOL_ML; auto.
+          unfold well_formed_closed in *. simpl.
+          eapply wf_increase_term with (n' := 1) in E2 as H4'. 2: lia.
+          eapply closed_term_FOL_ML in H4'.
+          separate. simpl in E0, E3. do 4 rewrite andb_true_r in E0, E3.
+          rewrite -> E0, -> E3.
+          rewrite -> bevar_subst_positive, -> bevar_subst_closed, -> closed_term_FOL_ML; auto.
+          eapply wf_increase_term. eassumption. lia.
+          now apply closed_term_FOL_ML.
+          now apply positive_term_FOL_ML.
         }
-        simpl in H.
-        rewrite HeqA, add_forall_prefix_subst in H.
-        simpl Nat.add in H.
+        simpl in H0.
+        rewrite -> HeqA, -> add_forall_prefix_subst in H0.
+        simpl Nat.add in H0.
         replace (bevar_subst
               (ex ,
                @patt_equal sig definedness_syntax
@@ -1360,25 +1101,32 @@ Section FOL_ML_correspondence.
                        (Acc $ patt_bound_evar x)%ml) 
                     (make_list1 n) (start $ patt_bound_evar (S n))%ml) (convert_term h) (S n))
                  BoundVarSugar.b0)) in H by auto.
-        rewrite subst_make_list in H. 2: lia.
-        simpl in H. rewrite HIND in H. break_match_hyp.
+        simpl in H0.
+        rewrite subst_make_list in H0. lia.
+        simpl in H0. rewrite HIND in H0. break_match_hyp.
         + lia.
-        + exact H.
+        + exact H0.
         + lia.
 
         (** asserted hypotheses *)
-        + intros. simpl. rewrite HIND. erewrite bevar_subst_identity.
-          auto. 2: { apply wf_term_FOL_ML. inversion H0. simpl_existT. subst. apply H4. }
+        + apply wf_ex_to_wf_body. unfold well_formed, well_formed_closed in *.
+          do 2 separate. simpl in E0, E3.
+          do 4 rewrite andb_true_r in E0, E3. simpl. now rewrite -> E0, -> E3.
+        + intros. simpl. rewrite HIND. erewrite well_formed_bevar_subst.
+          auto.
+          2: { apply closed_term_FOL_ML. inversion H0. separate. eassumption. }
           lia.
-        + constructor. auto.
-          apply term_mu_free.
+        + simpl. now rewrite -> HMUF, -> term_mu_free.
         + unfold well_formed, well_formed_closed in *.
-          simpl. apply eq_sym, andb_true_eq in WFS. destruct WFS. rewrite <- H, <- H2.
-          simpl. apply wf_FOL_ML_term. inversion H0. simpl_existT. subst. apply H6.
+          simpl. apply eq_sym, andb_true_eq in WFS. destruct WFS.
+          rewrite <- H2, <- H3.
+          simpl. rewrite -> positive_term_FOL_ML, -> closed_term_FOL_ML; auto.
+          separate. auto.
   Unshelve.
-    ** intros. apply IH; auto. constructor 2; auto.
-    ** inversion H0. simpl_existT. subst. auto.
-    ** exact 0.
+    4-7: exact 0.
+    ** auto.
+    ** intros. apply H; auto. constructor 2; auto.
+    ** now separate.
   Qed.
 
   Theorem arrow_1 : forall (φ : form) (Γ : list form), 
@@ -1387,26 +1135,29 @@ Section FOL_ML_correspondence.
     from_FOL_theory Γ ⊢_ML convert_form φ.
   Proof.
     intros φ Γ IH. induction IH; intros.
-    * apply hypothesis. 2: now apply in_theory. now apply wf_FOL_ML.
+    * apply hypothesis. now apply wf_form_FOL_ML. now apply in_FOL_theory.
     * simpl. apply P1; auto.
     * apply P2; auto.
     * apply P3; auto.
     * eapply Modus_ponens. 3: exact IHIH1. 3: exact IHIH2. all: auto.
-      inversion H0. subst. auto.
+      simpl in i0. separate. auto.
     * simpl.
-      epose proof (term_functionality t Γ H0).
-      pose proof (exists_functional_subst (convert_form φ) (convert_term t) (from_FOL_theory Γ)).
-      simpl in H1. rewrite bevar_subst_corr_form.
-      eapply and_impl_patt2. 4: exact H1. 4: exact H2.
-      all: apply wf_FOL_ML in H as H';auto.
-      - simpl in H. clear H2 H1. unfold well_formed in *.
-        apply andb_true_iff. apply andb_true_iff in H'. destruct H'.
-        split.
-        + simpl in *. now rewrite positive_term_FOL_ML.
-        + unfold well_formed_closed. simpl.
-          rewrite wf_term_FOL_ML; auto. eapply wf_increase_term. exact H0. lia.
-      - rewrite <- bevar_subst_corr_form. apply wf_FOL_ML. inversion H. subst.
-        apply wf_form_subst; auto. auto.
+      epose proof (term_functionality t Γ i0).
+      pose proof (@exists_functional_subst _ _ (convert_form φ) (convert_term t) (from_FOL_theory Γ)).
+      simpl in H0. rewrite bevar_subst_corr_form; auto.
+      eapply and_impl_patt2. 4: exact H. 4: apply H0.
+      all: unfold well_formed, well_formed_closed; simpl.
+      all: try rewrite -> closed_term_FOL_ML, -> positive_term_FOL_ML; auto.
+      apply wf_increase_term with (n := 0); auto.
+      2: try rewrite -> closed_form_FOL_ML, -> positive_form_FOL_ML; auto.
+      rewrite -> bevar_subst_well_formedness, -> well_formed_positive_bevar_subst.
+      auto.
+      1, 6: apply form_mu_free.
+      apply positive_form_FOL_ML.
+      apply positive_term_FOL_ML.
+      apply closed_form_FOL_ML; auto.
+      apply closed_term_FOL_ML; auto.
+      apply wf_ex_to_wf_body. apply wf_form_FOL_ML in i. exact i.
     * simpl. rewrite quantify_form_correspondence. eapply Ex_gen; auto.
       apply form_vars_free_vars_notin. auto.
   Qed.
@@ -1416,7 +1167,7 @@ End FOL_ML_correspondence.
 
 Section tests.
 
-  Inductive PA_funcs : Type :=
+  Inductive PA_funcs : Set :=
     Zero : PA_funcs
   | Succ : PA_funcs
   | Plus : PA_funcs
@@ -1435,7 +1186,7 @@ Section tests.
    | Mult => 2
    end.
 
-  Inductive PA_preds : Type :=
+  Inductive PA_preds : Set :=
     Eq : PA_preds.
 
   Theorem pa_preds_eqdec : EqDecision PA_preds.
@@ -1484,7 +1235,6 @@ Section tests.
      Definedness.inj := sym_import_definedness;
   |}.
 
-  Compute (add_forall_prefix 2) (patt_bott).
   Goal axiom (AxFun Mult) = patt_forall (patt_forall (patt_exists (patt_equal 
              (patt_app (patt_app (patt_sym (sym_fun Mult)) (patt_bound_evar 2)) (patt_bound_evar 1))
              (patt_bound_evar 0)))).
